Logic/Modal/Standard/Kripke/Grz_Completeness.lean
@@ -1,0 +1,286 @@
+import Logic.Modal.Standard.Kripke.Grz
+import Logic.Modal.Standard.Kripke.GL.Completeness
+
+namespace LO.Modal.Standard
+
+namespace Kripke
+
+open System
+open Kripke
+open Formula (atom)
+open Formula.Kripke
+
+variable {α : Type u} [Inhabited α] [DecidableEq α]
+variable {F : Kripke.Frame}
+
+
+abbrev GrzCanonicalFrame := CanonicalFrame (α := α) 𝐆𝐫𝐳
+abbrev GrzCanonicalModel := CanonicalModel (α := α) 𝐆𝐫𝐳
+
+-- TODO: Too slow
+set_option maxHeartbeats 1000000 in
+abbrev GrzFilteredFrame (p : Formula α) : Kripke.FiniteFrame where
+  World := FilterEqvQuotient GrzCanonicalModel ((𝒮 p).toSet)
+  World_finite := by apply FilterEqvQuotient.finite; simp;
+  Rel := Quotient.lift₂
+    (λ X Y =>
+      (∀ q ∈ □''⁻¹(𝒮 p), □q ∈ X.theory → □q ∈ Y.theory) ∧
+      ((∀ q ∈ □''⁻¹(𝒮 p), □q ∈ Y.theory → □q ∈ X.theory) → ∀ q ∈ □''⁻¹(𝒮 p), q ∈ X.theory ↔ q ∈ Y.theory)
+    )
+    (by
+      intro X₁ Y₁ X₂ Y₂ hX hY;
+      simp only [Set.eq_prebox_premultibox_one, Set.mem_preimage, Function.iterate_one, Finset.mem_coe, eq_iff_iff];
+      constructor;
+      . rintro ⟨h₁, h₂⟩;
+        constructor;
+        . intro q _ hq;
+          have : □q ∈ X₁.theory := filter_truthlemma (by simpa only) |>.mpr hq;
+          have : □q ∈ Y₁.theory := h₁ q (by assumption) this;
+          exact filter_truthlemma (by simpa only) |>.mp this;
+        . intro h q _;
+          constructor;
+          . intro hq;
+            have : q ∈ X₁.theory := filter_truthlemma (by simpa only) |>.mpr hq;
+            have : q ∈ Y₁.theory := h₂ ?_ q (by assumption) |>.mp this;
+            exact filter_truthlemma (by simpa only) |>.mp this;
+            intro q _ hq;
+            have : □q ∈ Y₂.theory := filter_truthlemma (by simpa only) |>.mp hq;
+            have : □q ∈ X₂.theory := h q (by assumption) this;
+            exact filter_truthlemma (by simpa only) |>.mpr this;
+          . intro hq;
+            have : q ∈ Y₁.theory := filter_truthlemma (by simpa only) |>.mpr hq;
+            have : q ∈ X₁.theory := h₂ ?_ q (by assumption) |>.mpr this;
+            exact filter_truthlemma (by simpa only) |>.mp this;
+            intro q _ hq;
+            have : □q ∈ Y₂.theory := filter_truthlemma (by simpa only) |>.mp hq;
+            have : □q ∈ X₂.theory := h q (by assumption) this;
+            exact filter_truthlemma (by simpa only) |>.mpr this;
+      . rintro ⟨h₁, h₂⟩;
+        constructor;
+        . intro q _ hq;
+          have : □q ∈ X₂.theory := filter_truthlemma (by simpa only) |>.mp hq;
+          have : □q ∈ Y₂.theory := h₁ q (by assumption) this;
+          exact filter_truthlemma (by simpa only) |>.mpr this;
+        . intro h q _;
+          constructor;
+          . intro hq;
+            have : q ∈ X₂.theory := filter_truthlemma (by simpa only) |>.mp hq;
+            have : q ∈ Y₂.theory := h₂ ?_ q (by assumption) |>.mp this;
+            exact filter_truthlemma (by simpa only) |>.mpr this;
+            intro q _ hq;
+            have : □q ∈ Y₁.theory := filter_truthlemma (by simpa only) |>.mpr hq;
+            have : □q ∈ X₁.theory := h q (by assumption) this;
+            exact filter_truthlemma (by simpa only) |>.mp this;
+          . intro hq;
+            have : q ∈ Y₂.theory := filter_truthlemma (by simpa only) |>.mp hq;
+            have : q ∈ X₂.theory := h₂ ?_ q (by assumption) |>.mpr this;
+            exact filter_truthlemma (by simpa only) |>.mpr this;
+            intro q _ hq;
+            have : □q ∈ Y₁.theory := filter_truthlemma (by simpa only) |>.mpr hq;
+            have : □q ∈ X₁.theory := h q (by assumption) this;
+            exact filter_truthlemma (by simpa only) |>.mp this;
+    )
+
+lemma GrzFilteredFrame.def_rel {p : Formula α} {X Y : GrzCanonicalFrame.World} :
+  ((GrzFilteredFrame p).Rel ⟦X⟧ ⟦Y⟧) ↔
+  (
+    (∀ q ∈ □''⁻¹(𝒮 p), □q ∈ X.theory → □q ∈ Y.theory) ∧
+    ((∀ q ∈ □''⁻¹(𝒮 p), □q ∈ Y.theory → □q ∈ X.theory) → ∀ q ∈ □''⁻¹(𝒮 p), q ∈ X.theory ↔ q ∈ Y.theory)
+  )
+  := by simp;
+
+lemma GrzFilteredFrame.reflexive {p : Formula α} : Reflexive (GrzFilteredFrame p).Rel := by
+  intro QX;
+  obtain ⟨X, hX⟩ := Quotient.exists_rep QX; subst hX;
+  simp_all;
+
+lemma GrzFilteredFrame.transitive {p : Formula α} : Transitive (GrzFilteredFrame p).Rel := by
+  intro QX QY QZ RXY RYZ;
+  obtain ⟨X, hX⟩ := Quotient.exists_rep QX; subst hX;
+  obtain ⟨Y, hY⟩ := Quotient.exists_rep QY; subst hY;
+  obtain ⟨Z, hZ⟩ := Quotient.exists_rep QZ; subst hZ;
+  replace ⟨hXY₁, hXY₂⟩ := RXY;
+  replace ⟨hYZ₁, hYZ₂⟩ := RYZ;
+  constructor;
+  . intro q hs hq;
+    exact hYZ₁ q hs $ hXY₁ q hs hq
+  . intro h;
+    have hX := hXY₂ $ by
+      intro q hs hq;
+      exact h q hs $ hYZ₁ q hs hq;
+    have hZ := hYZ₂ $ by
+      intro q hs hq;
+      exact hXY₁ q hs $ h q hs hq
+    intro q hq;
+    exact Iff.trans (hX q hq) (hZ q hq);
+
+lemma GrzFilteredFrame.antisymm {p : Formula α} : Antisymmetric (GrzFilteredFrame p).Rel := by
+  intro QX QY RXY RYX;
+  obtain ⟨X, hX⟩ := Quotient.exists_rep QX; subst hX;
+  obtain ⟨Y, hY⟩ := Quotient.exists_rep QY; subst hY;
+  have := RXY.2 RYX.1;
+  sorry;
+
+abbrev GrzFilteredModel (p : Formula α) : Kripke.Model α where
+  Frame := GrzFilteredFrame p
+  Valuation := StandardFilterationValuation GrzCanonicalModel ((𝒮 p).toSet)
+
+-- TODO: syntactical proof
+private lemma K4_lemma1 {q : Formula α} : 𝐊𝟒 ⊢! (□q ⟶ □(q ⟶ □q)) := by
+  by_contra hC;
+  have := (not_imp_not.mpr $ K4_complete (α := α) |>.complete) hC;
+  simp only [ValidOnFrameClass.models_iff, ValidOnFrameClass, Set.mem_setOf_eq, Transitive,
+    ValidOnFrame.models_iff, ValidOnFrame, ValidOnModel.iff_models, ValidOnModel,
+    Satisfies.iff_models, Satisfies, not_forall, Classical.not_imp] at this;
+  obtain ⟨F, F_trans, V, x, h, y, Rxy, _, z, Ryz, j⟩ := this;
+  have := h (F_trans Rxy Ryz);
+  contradiction;
+
+open System System.FiniteContext MaximalConsistentTheory in
+private lemma Grz_truthlemma.lemma1
+  {q : Formula α}
+  {X : (CanonicalModel 𝐆𝐫𝐳).World} (h : □(q ⟶ □q) ∉ X.theory) : (𝐆𝐫𝐳)-Consistent ({□(q ⟶ □q), ~q} ∪ (□''□''⁻¹X.theory)) := by
+  by_contra hC;
+  obtain ⟨Γ, hΓ₁, hΓ₂⟩ := Context.provable_iff.mp hC;
+  have := toₛ! hΓ₂;
+  have : 𝐆𝐫𝐳 ⊢! ⋀(Γ.remove (~q)) ⋏ ~q ⟶ ⊥ := imply_left_remove_conj! (p := ~q) this;
+  have : 𝐆𝐫𝐳 ⊢! ⋀(Γ.remove (~q)) ⟶ ~q ⟶ ⊥ := and_imply_iff_imply_imply'!.mp this;
+  have : 𝐆𝐫𝐳 ⊢! ⋀(Γ.remove (~q)) ⟶ q := imp_trans''! this $ imp_trans''! (and₂'! neg_equiv!) dne!
+  have : 𝐆𝐫𝐳 ⊢! ⋀((Γ.remove (~q)).remove (□(q ⟶ □q))) ⋏ (□(q ⟶ □q)) ⟶ q := imply_left_remove_conj! (p := □(q ⟶ □q)) this;
+  have : 𝐆𝐫𝐳 ⊢! ⋀((Γ.remove (~q)).remove (□(q ⟶ □q))) ⟶ (□(q ⟶ □q) ⟶ q)  := and_imply_iff_imply_imply'!.mp this;
+  have : 𝐆𝐫𝐳 ⊢! □⋀((Γ.remove (~q)).remove (□(q ⟶ □q))) ⟶ □(□(q ⟶ □q) ⟶ q) := imply_box_distribute'! this;
+  have : 𝐆𝐫𝐳 ⊢! □⋀((Γ.remove (~q)).remove (□(q ⟶ □q))) ⟶ q := imp_trans''! this axiomGrz!;
+  have : 𝐆𝐫𝐳 ⊢! □□⋀((Γ.remove (~q)).remove (□(q ⟶ □q))) ⟶ □q := imply_box_distribute'! this;
+  have : 𝐆𝐫𝐳 ⊢! □⋀((Γ.remove (~q)).remove (□(q ⟶ □q))) ⟶ □q := imp_trans''! axiomFour! this;
+  have : 𝐆𝐫𝐳 ⊢! ⋀□'((Γ.remove (~q)).remove (□(q ⟶ □q))) ⟶ □q := imp_trans''! collect_box_conj! this;
+  have : 𝐆𝐫𝐳 ⊢! ⋀□'((Γ.remove (~q)).remove (□(q ⟶ □q))) ⟶ (□(q ⟶ □q)) := imp_trans''! this (reducible_K4_Grz K4_lemma1)
+
+  have : X.theory *⊢[𝐆𝐫𝐳]! (□(q ⟶ □q)) := by
+    apply Context.provable_iff.mpr;
+    use (□'List.remove (□(q ⟶ □q)) (List.remove (~q) Γ));
+    constructor;
+    . intro r hr; simp at hr;
+      obtain ⟨s, hs, rfl⟩ := hr;
+      have ⟨s_mem', hs₁⟩ := List.mem_remove_iff.mp hs;
+      have ⟨s_mem, hs₂⟩ := List.mem_remove_iff.mp s_mem';
+      clear hs s_mem';
+      have := hΓ₁ s s_mem;
+      simp at this;
+      rcases this with ((rfl | rfl) | ⟨s, hs, rfl⟩);
+      . contradiction;
+      . contradiction;
+      . apply membership_iff.mpr;
+        apply axiomFour'!;
+        apply membership_iff.mp;
+        assumption;
+    . assumption;
+
+  have : □(q ⟶ □q) ∈ X.theory := membership_iff.mpr this;
+  contradiction;
+
+open System System.FiniteContext MaximalConsistentTheory in
+private lemma Grz_truthlemma.lemma2
+  {q : Formula α}
+  {X : (CanonicalModel 𝐆𝐫𝐳).World} (h : □q ∉ X.theory) : (𝐆𝐫𝐳)-Consistent ({□(q ⟶ □q), ~q} ∪ (□''□''⁻¹X.theory)) := by
+  by_contra hC;
+  obtain ⟨Γ, hΓ₁, hΓ₂⟩ := Context.provable_iff.mp hC;
+  have := toₛ! hΓ₂;
+  have : 𝐆𝐫𝐳 ⊢! ⋀(Γ.remove (~q)) ⋏ ~q ⟶ ⊥ := imply_left_remove_conj! (p := ~q) this;
+  have : 𝐆𝐫𝐳 ⊢! ⋀(Γ.remove (~q)) ⟶ ~q ⟶ ⊥ := and_imply_iff_imply_imply'!.mp this;
+  have : 𝐆𝐫𝐳 ⊢! ⋀(Γ.remove (~q)) ⟶ q := imp_trans''! this $ imp_trans''! (and₂'! neg_equiv!) dne!
+  have : 𝐆𝐫𝐳 ⊢! ⋀((Γ.remove (~q)).remove (□(q ⟶ □q))) ⋏ (□(q ⟶ □q)) ⟶ q := imply_left_remove_conj! (p := □(q ⟶ □q)) this;
+  have : 𝐆𝐫𝐳 ⊢! ⋀((Γ.remove (~q)).remove (□(q ⟶ □q))) ⟶ (□(q ⟶ □q) ⟶ q)  := and_imply_iff_imply_imply'!.mp this;
+  have : 𝐆𝐫𝐳 ⊢! □⋀((Γ.remove (~q)).remove (□(q ⟶ □q))) ⟶ □(□(q ⟶ □q) ⟶ q) := imply_box_distribute'! this;
+  have : 𝐆𝐫𝐳 ⊢! □⋀((Γ.remove (~q)).remove (□(q ⟶ □q))) ⟶ q := imp_trans''! this axiomGrz!;
+  have : 𝐆𝐫𝐳 ⊢! □□⋀((Γ.remove (~q)).remove (□(q ⟶ □q))) ⟶ □q := imply_box_distribute'! this;
+  have : 𝐆𝐫𝐳 ⊢! □⋀((Γ.remove (~q)).remove (□(q ⟶ □q))) ⟶ □q := imp_trans''! axiomFour! this;
+  have : 𝐆𝐫𝐳 ⊢! ⋀□'((Γ.remove (~q)).remove (□(q ⟶ □q))) ⟶ □q := imp_trans''! collect_box_conj! this;
+
+  have : X.theory *⊢[𝐆𝐫𝐳]! (□q) := by
+    apply Context.provable_iff.mpr;
+    use (□'List.remove (□(q ⟶ □q)) (List.remove (~q) Γ));
+    constructor;
+    . intro r hr; simp at hr;
+      obtain ⟨s, hs, rfl⟩ := hr;
+      have ⟨s_mem', hs₁⟩ := List.mem_remove_iff.mp hs;
+      have ⟨s_mem, hs₂⟩ := List.mem_remove_iff.mp s_mem';
+      clear hs s_mem';
+      have := hΓ₁ s s_mem;
+      simp at this;
+      rcases this with ((rfl | rfl) | ⟨s, hs, rfl⟩);
+      . contradiction;
+      . contradiction;
+      . apply membership_iff.mpr;
+        apply axiomFour'!;
+        apply membership_iff.mp;
+        assumption;
+    . assumption;
+
+  have : □q ∈ X.theory := membership_iff.mpr this;
+  contradiction;
+
+open Formula MaximalConsistentTheory
+
+lemma Grz_truthlemma
+  {p : Formula α} {X : (CanonicalModel 𝐆𝐫𝐳).World} {q : Formula α} (hq : q ∈ 𝒮 p) :
+  Satisfies (GrzFilteredModel p) ⟦X⟧ q ↔ q ∈ X.theory := by
+  induction q using Formula.rec' generalizing X with
+  | hbox q ih =>
+    constructor;
+    . contrapose;
+      intro h;
+      obtain ⟨Y, hY⟩ := lindenbaum (Λ := 𝐆𝐫𝐳) (T := ({□(q ⟶ □q), ~q} ∪ (□''□''⁻¹X.theory))) $ Grz_truthlemma.lemma2 h;
+      simp [Satisfies];
+      use ⟦Y⟧;
+      constructor;
+      . apply GrzFilteredFrame.def_rel.mpr;
+        simp [Set.insert_subset_iff] at hY;
+        have ⟨⟨mem_q₁_Y, nmem_q_Y⟩, hY₂⟩ := hY;
+        constructor;
+        . intro r _ _; apply hY₂; simpa;
+        . by_contra hC;
+          push_neg at hC;
+          obtain ⟨hr, r, hr₁, (⟨hr₂, hr₃⟩ | ⟨hr₂, hr₃⟩)⟩ := hC;
+          . simp at hr₁;
+            sorry;
+          . have := @hr r (by sorry) (by sorry);
+            sorry;
+      . apply ih (by aesop) |>.not.mpr;
+        apply iff_mem_neg.mp;
+        apply hY;
+        simp;
+    . intro bq_mem_X QY RXY;
+      obtain ⟨Y, hY⟩ := Quotient.exists_rep QY; subst hY;
+      have ⟨h₁, _⟩ := GrzFilteredFrame.def_rel.mp RXY; simp at h₁;
+      have := h₁ q hq bq_mem_X;
+      apply @ih Y (Subformulas.mem_box hq) |>.mpr;
+      sorry;
+      -- have ⟨q_mem_Y, _⟩ := h₁ q hq bq_mem_X;
+      -- exact ih (by aesop) |>.mpr q_mem_Y;
+  | _ =>
+    sorry;
+    -- simp_all [Satisfies, StandardFilterationValuation];
+    -- try aesop;
+
+private lemma Grz_completeAux {p : Formula α} : ReflexiveTransitiveAntisymmetricFrameClass.{u}ꟳ# ⊧ p → 𝐆𝐫𝐳 ⊢! p := by
+  contrapose;
+  intro h;
+  apply exists_finite_frame.mpr;
+  use (GrzFilteredFrame p);
+  constructor;
+  . refine ⟨GrzFilteredFrame.reflexive, GrzFilteredFrame.transitive, GrzFilteredFrame.antisymm⟩;
+  . simp [Formula.Kripke.ValidOnFrame, Formula.Kripke.ValidOnModel];
+    obtain ⟨X, hX⟩ := lindenbaum (Λ := 𝐆𝐫𝐳) (T := {~p}) (Theory.unprovable_iff_singleton_neg_consistent.mp h);
+    use (GrzFilteredModel p).Valuation, ⟦X⟧;
+    apply Grz_truthlemma (by simp) |>.not.mpr;
+    apply MaximalConsistentTheory.iff_mem_neg.mp;
+    simpa using hX;
+
+instance Grz_complete : Complete (𝐆𝐫𝐳 : DeductionParameter α) ReflexiveTransitiveAntisymmetricFrameClass.{u}ꟳ# := ⟨Grz_completeAux⟩
+
+instance : FiniteFrameProperty (α := α) 𝐆𝐫𝐳 ReflexiveTransitiveAntisymmetricFrameClass where
+
+
+end Kripke
+
+end LO.Modal.Standard
